Manual fix on things.

out/ERC20Function.sol
@@ -1,4 +1,6 @@
-function transferFromSimple(uint256 from, uint256 to, uint256 value) public virtual returns (bool, uint256, uint256) {
+function transferFromSimple(
+  uint256 from, uint256 to, uint256 value
+) public virtual returns (bool, uint256, uint256) {
 	if (from < value) {
     return (false, from, to);
 	}
