Generated/ERC20simple/ERC20Shim/Common/if_5295847412656974480_user.lean
@@ -10,7 +10,11 @@ section
 
 open Clear EVMState Ast Expr Stmt FunctionDefinition State Interpreter ExecLemmas OutOfFuelLemmas Abstraction YulNotation PrimOps ReasoningPrinciple Utilities 
 
-def A_if_5295847412656974480 (s₀ s₉ : State) : Prop := sorry
+def A_if_5295847412656974480 (s₀ s₉ : State) : Prop :=
+  (if s₀["expr_2"]!! = 0
+   then s₀
+   else 🚪s₀⟦"expr_3"↦0⟧⟦"expr_201_component"↦0⟧⟦"_3"↦s₀["var_from"]!!⟧⟦"expr_4"↦s₀["var_from"]!!⟧⟦"expr_201_component_1"↦s₀["var_from"]!!⟧⟦"_4"↦s₀["var_to"]!!⟧⟦"expr_5"↦s₀["var_to"]!!⟧⟦"expr_component"↦s₀["var_to"]!!⟧⟦"var"↦0⟧⟦"var_1"↦s₀["var_from"]!!⟧⟦"var_2"↦s₀["var_to"]!!⟧) =
+  s₉
 
 lemma if_5295847412656974480_abs_of_concrete {s₀ s₉ : State} :
   Spec if_5295847412656974480_concrete_of_code s₀ s₉ →
